change division_ring axiom from `mul_one` to `one_mul`

library/init/algebra/field.lean
@@ -18,8 +18,8 @@ set_option old_structure_cmd true
 
 class division_ring (α : Type u) extends
   add_group α, semigroup α, has_one α, distrib α, has_inv α, zero_ne_one_class α :=
-(mul_one : ∀ a : α, a * 1 = a)
-(mul_inv_cancel : ∀ {a : α}, a ≠ 0 → a * a⁻¹ = 1)
+(one_mul : ∀ a : α, 1 * a = a)
+(inv_mul_cancel : ∀ {a : α}, a ≠ 0 → a⁻¹ * a = 1)
 (inv_zero : (0 : α)⁻¹ = 0)
 
 variable {α : Type u}
@@ -40,8 +40,8 @@ rfl
 division_ring.inv_zero α
 
 @[simp]
-lemma mul_inv_cancel {a : α} (h : a ≠ 0) : a * a⁻¹ = 1 :=
-division_ring.mul_inv_cancel h
+lemma inv_mul_cancel {a : α} (h : a ≠ 0) : a⁻¹ * a = 1 :=
+division_ring.inv_mul_cancel h
 
 lemma division_ring.zero_mul (a : α) : 0 * a = 0 :=
 have 0 * a + 0 = 0 * a + 0 * a, from calc
@@ -55,45 +55,44 @@ have a * 0 + 0 = a * 0 + a * 0, from calc
            ... = a * 0 + a * 0 : by rw left_distrib,
 show a * 0 = 0, from (add_left_cancel this).symm
 
-
-@[simp] lemma div_zero (a : α) : a / 0 = (0:α) :=
-calc
-  a / 0 = (a:α) * 0⁻¹ : by rw division_def
-    ... = a * 0       : by rw inv_zero
-    ... = (0:α)       : by rw division_ring.mul_zero
-
 lemma inv_ne_zero {a : α} (h : a ≠ 0) : a⁻¹ ≠ 0 :=
 assume : a⁻¹ = 0,
-have 0 = (1 : α), by rw [← mul_inv_cancel h, this, division_ring.mul_zero],
+have 0 = (1 : α), by rw [← inv_mul_cancel h, this, division_ring.zero_mul],
 zero_ne_one this
 
 -- note: integral domain has a "mul_ne_zero". α commutative division ring is an integral
 -- domain, but let's not define that class for now.
 lemma division_ring.mul_ne_zero {a b : α} (ha : a ≠ 0) (hb : b ≠ 0) : a * b ≠ 0 :=
 assume : a * b = 0,
-have   a * 1 = 0, by rw [← mul_inv_cancel hb, ← mul_assoc, this, division_ring.zero_mul],
-have   a = 0, by rwa division_ring.mul_one at this,
-absurd this ha
+have   1 * b = 0, by rw [← inv_mul_cancel ha, mul_assoc, this, division_ring.mul_zero],
+have   b = 0, by rwa division_ring.one_mul at this,
+absurd this hb
 
 @[simp]
-lemma inv_mul_cancel {a : α} (h : a ≠ 0) : a⁻¹ * a = 1 :=
-have a⁻¹ * a ≠ 0, from division_ring.mul_ne_zero (inv_ne_zero h) h,
-calc a⁻¹ * a =  (a⁻¹ * a) * ((a⁻¹ * a) * (a⁻¹ * a)⁻¹) :
-  by rw [mul_inv_cancel this, division_ring.mul_one]
-... = (a⁻¹ * a) * (a⁻¹ * a)⁻¹ :
-  by rw [← mul_assoc, ← mul_assoc, mul_assoc _ _ (a⁻¹), mul_inv_cancel h, division_ring.mul_one]
-... = 1 : by rw mul_inv_cancel this
+lemma mul_inv_cancel {a : α} (h : a ≠ 0) : a * a⁻¹ = 1 :=
+have a * a⁻¹ ≠ 0, from division_ring.mul_ne_zero h (inv_ne_zero h) ,
+calc a * a⁻¹ = (a * a⁻¹)⁻¹ * (a * a⁻¹) * (a * a⁻¹) :
+  by rw [inv_mul_cancel this, division_ring.one_mul]
+... = (a * a⁻¹)⁻¹ * (a * a⁻¹) :
+  by rw [mul_assoc, mul_assoc, ← mul_assoc (a⁻¹), inv_mul_cancel h, division_ring.one_mul]
+... = 1 : by rw inv_mul_cancel this
 
-lemma division_ring.one_mul (a : α) : 1 * a = a :=
+lemma division_ring.mul_one (a : α) : a * 1 = a :=
 classical.by_cases
-  (λ ha0 : a = 0, by rw [ha0, division_ring.mul_zero])
+  (λ ha0 : a = 0, by rw [ha0, division_ring.zero_mul])
   (λ ha0 : a ≠ 0,
-      by rw [← mul_inv_cancel ha0, mul_assoc,
-        inv_mul_cancel ha0, division_ring.mul_one])
+      by rw [← inv_mul_cancel ha0, ← mul_assoc,
+        mul_inv_cancel ha0, division_ring.one_mul])
 
 instance division_ring.to_ring : ring α :=
-{ one_mul := division_ring.one_mul,
+{ mul_one := division_ring.mul_one,
   ..show division_ring α, by apply_instance }
+
+@[simp] lemma div_zero (a : α) : a / 0 = (0:α) :=
+calc
+  a / 0 = (a:α) * 0⁻¹ : by rw division_def
+    ... = a * 0       : by rw inv_zero
+    ... = (0:α)       : by rw division_ring.mul_zero
 
 @[simp]
 lemma one_div_eq_inv (a : α) : 1 / a = a⁻¹ :=
@@ -102,11 +101,13 @@ division_ring.one_mul a⁻¹
 lemma inv_eq_one_div (a : α) : a⁻¹ = 1 / a :=
 by simp
 
-lemma mul_one_div_cancel {a : α} (h : a ≠ 0) : a * (1 / a) = 1 :=
+lemma one_div_mul_cancel {a : α} (h : a ≠ 0) : (1 / a) * a = 1 :=
 by simp [h]
 
 lemma one_div_ne_zero {a : α} (h : a ≠ 0) : 1 / a ≠ 0 :=
-inv_eq_one_div a ▸ inv_ne_zero h
+assume : 1 / a = 0,
+have 0 = (1:α), by rw [← one_div_mul_cancel h, this, zero_mul],
+absurd this zero_ne_one
 
 local attribute [simp]
 division_def mul_comm mul_assoc
@@ -115,8 +116,8 @@ mul_left_comm inv_mul_cancel
 lemma div_eq_mul_one_div (a b : α) : a / b = a * (1 / b) :=
 by simp
 
-lemma one_div_mul_cancel {a : α} (h : a ≠ 0) : (1 / a) * a = 1 :=
-by rw [division_def, mul_assoc, inv_mul_cancel h, division_ring.one_mul]
+lemma mul_one_div_cancel {a : α} (h : a ≠ 0) : a * (1 / a) = 1 :=
+by simp [h]
 
 lemma div_self {a : α} (h : a ≠ 0) : a / a = 1 :=
 by simp [h]
@@ -269,7 +270,7 @@ by simp [hc]
 end division_ring
 
 class field (α : Type u) extends comm_ring α, has_inv α, zero_ne_one_class α :=
-(mul_inv_cancel : ∀ {a : α}, a ≠ 0 → a * a⁻¹ = 1)
+(inv_mul_cancel : ∀ {a : α}, a ≠ 0 → a⁻¹ * a = 1)
 (inv_zero : (0 : α)⁻¹ = 0)
 
 section field
